src/Pipit.Sugar.Check.fst
@@ -36,12 +36,12 @@ let contract_system_induct_k1 (#t: table) (#c: context t) (#a: t.ty) (contr: _co
   SI.induct1 (SX.system_of_contract contr.rely contr.guar contr.impl)
 
 
-let stream_of_contract1 (#t: table) (#a #b: t.ty) (contr: _contract t [a] b): s t a -> s t b =
+let stream_of_contract1 (#t: table) (#a #b: t.ty) (contr: _contract t [a] b { XC.check_contract_definition PM.check_mode_all contr.rely contr.guar contr.impl }): s t a -> s t b =
   let rely = XC.bless contr.rely in
   let guar = XC.bless contr.guar in
   let impl = XC.bless contr.impl in
-  // TODO:ADMIT: requires contract_check
   let e = XContract PM.PSUnknown rely guar impl in
+  // TODO:ADMIT: requires contract_check
   assume (XC.check' PM.check_mode_valid e);
   stream_of_exp1 e
 
@@ -49,6 +49,7 @@ let stream_of_contract1 (#t: table) (#a #b: t.ty) (contr: _contract t [a] b): s 
 let exp_of_stream0 (#t: table) (#ty: t.ty) (e: s t ty) : XCC.cexp t [] ty = exp_of_stream0 e
 let exp_of_stream1 (#t: table) (#a #b: t.ty) (f: s t a -> s t b) : XCC.cexp t [a] b = exp_of_stream1 f
 let exp_of_stream2 (#t: table) (#a #b #c: t.ty) (f: s t a -> s t b -> s t c) : XCC.cexp t [a; b] c = exp_of_stream2 f
+let exp_of_stream3 (#t: table) (#a #b #c #d: t.ty) (f: s t a -> s t b -> s t c -> s t d) : XCC.cexp t [a; b; c] d = exp_of_stream3 f
 
 
 let stream_of_checked0 (#t: table) (#a: t.ty) (e: exp t [] a { XC.check' PM.check_mode_all e }): s t a =
@@ -62,6 +63,10 @@ let stream_of_checked1 (#t: table) (#a #b: t.ty) (e: exp t [a] b { XC.check' PM.
 let stream_of_checked2 (#t: table) (#a #b #c: t.ty) (e: exp t [a; b] c { XC.check' PM.check_mode_all e }): s t a -> s t b -> s t c =
   let e' = XC.bless e in
   stream_of_exp2 e'
+
+let stream_of_checked3 (#t: table) (#a #b #c #d: t.ty) (e: exp t [a; b; c] d { XC.check' PM.check_mode_all e }): s t a -> s t b -> s t c -> s t d =
+  let e' = XC.bless e in
+  stream_of_exp3 e'
 
 
 let system_induct_k1 (#t: table) (#c: context t) (#a: t.ty) (e: XCC.cexp t c a): prop =
@@ -82,6 +87,14 @@ let lemma_check_system_induct_k (#t: table) (#c: context t) (#a: t.ty) (k: nat) 
   Lemma (requires (system_induct_k k e))
         (ensures  (XC.check' PM.check_mode_all e))
         [SMTPat (system_induct_k k e)]
+        =
+    // TODO:ADMIT: induction is sound
+    admit ()
+
+let lemma_check_contract_system_induct_k1 (#t: table) (#c: context t) (#a: t.ty) (contr: _contract t c a):
+  Lemma (requires (contract_system_induct_k1 contr))
+        (ensures  (XC.check_contract_definition PM.check_mode_all contr.rely contr.guar contr.impl))
+        [SMTPat (contract_system_induct_k1 contr)]
         =
     // TODO:ADMIT: induction is sound
     admit ()
